

<section>
  <title>The Chain Rule</title>
  <example>
    <statement>
      <p>
        Suppose we are given <m>A(t) = 1000 e^{0.149t}</m>.
        Find <m>A'(1)</m>.
      </p>
    </statement>
    <solution>
      <p>
        The main idea here is to apply the chain rule to <m>e^{0.149t}</m>.
        If
        it was just <m>e^t</m> we would use the basic rule, <m>\ddt e^t = e^t</m>,
        i.e.<nbsp />do nothing.
        Since we have <m>0.149t</m> <q>inside</q> of the
        exponent, we should use the chain rule.
        We start with the basic
        rule (do nothing in this case),
        we don't change the inside, and then
        we multiply by the derivative of the inside.
        I'll write this in two
        ways: (1) using an extra variable,
        <m>z</m>, like the book does, to label
        the inside function, (2) using colors and words to keep track of
        what's inside and what's outside.
        <em>You</em> don't need to write it
        both ways, choose what works best for you.
        <md>
          <mrow>\begin{aligned}\ddt e^z \amp  = \deriv{y}{z}\cdot \deriv{z}{t} \text{ where } y=e^z,\text{ and } z=0.149t\\
          \amp  = e^z\cdot (0.149)\\
          \amp  = e^{0.149t}(0.149)
          \end{aligned}</mrow>
          <mrow>\text{ or }  
          $\chain[(0.5ex,0.5ex)]{\ddt
          e^{0.149t}_{}}{e^{(\inside{0.149t})}_{}}{(0.149)}$</mrow>
        </md>
      </p>

      <p>
        Now we combine this with the rest of the formula for <m>A(t)</m> and
        evaluate at <m>t=1</m>
        <md>
          <mrow>A'(t) \amp  = 1000 e^{0.149t}(0.149)</mrow>
          <mrow>\amp  = 149e^{0.149t}</mrow>
          <mrow>A'(1) \amp  = 149e^{0.149}</mrow>
          <mrow>\amp  \approx 172.94</mrow>
        </md>
      </p>
    </solution>
  </example>

  <example>
    <statement>
      <p>
        Find the derivatives of

        <ol>
          <li>
            <p>
              <m>R = (q^3-5q+7)^5</m>
            </p>
          </li>

          <li>
            <p>
              <m>h(x) = \frac{17}{\sqrt{3+5x^2}}</m>
            </p>
          </li>
        </ol>
      </p>
    </statement>
    <solution>
      <p>
        For Chain Rule problems,
        we want to think of what is the
        <q>outside function</q>
        and what is the <q>inside function</q>,
        and we need each of these to be simple enough that we know how to find its derivatives.
        Sometimes it is best to think of the
        <q>outside function</q>
        as the last calculation you do.
      </p>

      <p>
        For (a), we see that the last calculation that would be done would
        be to take the fifth-power what is in the parentheses.
        Thus we'd
        have <m>z = q^3 -5q+7</m> and <m>R = z^5</m>.
        The Chain Rule gives us
        <md>
          <mrow>\begin{aligned}\deriv{R}{q} \amp  = \deriv{R}{z} \cdot \deriv{z}{q}, \text{ where } R  = z^5, z= q^3-5q+7\\
          \amp  = 5z^4\cdot (3q^2-5)\\
          \amp  = 5(q^3-5q+7)^4(3q^2-5)
          \end{aligned}</mrow>
          <mrow>\text{ or }   \chain{\ddq (q^3-5q+7)^5}
          {5(\inside{q^3-5q+7})^4} {(3q^2-5)}</mrow>
        </md>
      </p>

      <p>
        For (b), we need to rewrite the function, changing the
        radical in the denominator to a negative exponent:
        <m>h(x) = 17(3+5x^2)^{-1/2}</m>.
        Then we use the Power and Chain Rule
        Combined:
        <me>
          \chain{\ddx 17(3+5x^2)^{-1/2}} {17\left(-\tfrac{1}{2}\right)(\inside{3+5x^2})^{-3/2}} {(10x)}
        </me>
      </p>

      <p>
        We can clean this up, but please be clear in your head:
        we are done
        with the derivative at this point.
        The rest is algebra which
        <em>might</em> be useful, but you also might sometimes not want to do
        it, and in any case it's not the new part here.
        <md>
          <mrow>17\left(-\frac{1}{2}\right)(3+5x^2)^{-3/2} (10x)
          \amp  = -\frac{17(10)}{2} (3+5x^2)^{-3/2}x</mrow>
          <mrow>\amp  = \frac{85x}{(3+5x^2)^{3/2}}</mrow>
        </md>
      </p>
    </solution>
  </example>

  <example>
    <statement>
      <p>
        Find the derivatives of

        <ol>
          <li>
            <p>
              <m>y = 5e^{6x} +e^{-x}</m>
            </p>
          </li>

          <li>
            <p>
              <m>y = e^{3x^2-7x+11}</m>
            </p>
          </li>
        </ol>
      </p>
    </statement>
    <solution>
      <p>
        With exponential functions it's a little tricky to spot what
        <q>inside function</q> means.
        Basically, we should just learn with
        experience that for these, <q>inside</q> means what's on top.
        You can
        make this a little easier to see if you realize that the exponents
        are basically inside implied parentheses:
        <me>
          e^x = e^{(x)},
          e^{6x} = e^{(6x)},
          e^{-x} = e^{(-x)},
          e^{3x^2-7x+11} = e^{(3x^2-7x+11)},\ \text{ etc. }
        </me>
      </p>

      <p>
        Now <q>inside</q> really means inside,
        it's inside the parentheses.
        If
        you combine this with the Chain Rule you get the following pattern
        <md>
          <mrow>y \amp  = e^z,\ z=\text{ stuff } 
          \deriv{y}{x} \amp  = \deriv{y}{z}\cdot \deriv{z}{x}</mrow>
          <mrow>y \amp  = e^{\text{ (stuff) } } \implies y' = e^{\text{ (stuff) } } (\text{ stuff } )'</mrow>
        </md>
      </p>

      <p>
        We'll use this in both parts below.
      </p>

      <p>
        For (a), we use the Chain Rule on each of the terms, using the pattern
        above.
        Thus we get
        <md>
          <mrow>y' \amp  =(5e^{6x}+e^{-x})'</mrow>
          <mrow>\amp  = 5e^{(6x)}(6x)' + e^{(-x)}(-x)'</mrow>
          <mrow>\amp  = 5e^{6x}(6)+e^{-x}(-1)</mrow>
          <mrow>\amp  = 30e^{6x} - e^{-x}</mrow>
        </md>
      </p>

      <p>
        For (b), we use the pattern for Exponential Functions and Chain Rule Combined:
        <md>
          <mrow>y' \amp  = e^{\text{ (stuff) } } (\text{ stuff } )'</mrow>
          <mrow>y' \amp  =  e^{(3x^2-7x+11)}(3x^2-7x+11)'</mrow>
          <mrow>\amp  =  e^{(3x^2-7x+11)}(6x-7)</mrow>
          <mrow>\amp  = (6x-7)e^{3x^2-7x+11}</mrow>
        </md>
      </p>

      <p>
        Note: it's important that you include the parentheses around <m>6x-7</m>: Without them it's not right,
        and you will lose points.
      </p>
    </solution>
  </example>

  <example>
    <statement>
      <p>
        Find the derivative of <m>f(x) = \ln(x^2+5)</m>.
      </p>
    </statement>
    <solution>
      <p>
        Here we have: outside = <m>\ln()</m> and inside = <m>x^2+5</m>.
        <md>
          <mrow>\begin{aligned}\deriv{f}{x} \amp  = \deriv{f}{z} \cdot \deriv{z}{x} \text{ where } z=x^2+5\\
          \amp  = \frac{1}{z}\cdot (2x)\\
          \amp  = \frac{2x}{x^2+5}
          \end{aligned}</mrow>
          <mrow>\text{ or } \lnchain{\ddx \ln(x^2+5)}
          {\frac{1}{\inside{x^2+5}}} {(2x)}</mrow>
        </md>
      </p>

      <p>
        This gives us the pattern for natural logarithms with the Chain Rule:
        <me>
          y = \ln(\text{ stuff } ) \implies y' = \frac{1}{(\text{ stuff } )}
          (\text{ stuff } )' = \frac{(\text{ stuff } )'}{\text{ stuff } }
        </me>
      </p>
    </solution>
  </example>
</section>

