

<section>
  <title>Shortcuts for powers of <m>x</m>,
  constants, sums, and differences</title>
  <example>
    <statement>
      <p>
        Let <m>f(x)=3x^2-5x+8</m>.
        Find <m>f'(x)</m>.
      </p>
    </statement>
    <solution>
      <p>
        With practice, you can probably just write this down in one step:
        <me>
          f'(x) = 6x -5
        </me>
      </p>

      <p>
        But when you are still learning these steps, it might help to break it
        down more:
        <md>
          <mrow>f'(x) \amp  = \ddx (3x^2-5x+8) \amp \amp \text{ ``\(f'(x)\)'' means ``take the derivative'' }</mrow>
          <mrow>\amp   = \ddx (3x^2) - \ddx(5x) + \ddx(8) \amp \amp  \text{ apply the derivative across \(+\) and \(-\) signs }</mrow>
          <mrow>\amp   = 3\cdot 2x^1 - 5\cdot x^0 + 0  \amp \amp  \text{ ``constant multiple'', ``constant rule'' and ``power rule'' }</mrow>
          <mrow>\amp   = 6 x  - 5  \amp \amp  \text{ just cleaning up }</mrow>
        </md>
      </p>
    </solution>
  </example>

  <example>
    <statement>
      <ol>
        <li>
          <p>
            For <m>f(x)=6\sqrt{x}</m> find <m>f'(x)</m>.
          </p>
        </li>

        <li>
          <p>
            For <m>C(q) = q^{13}-\frac{5}{q^3}+7</m>, find the marginal cost.
          </p>
        </li>
      </ol>
    </statement>
    <solution>
      <p>
        <ol>
          <li>
            <p>
              Before taking the derivative of <m>\sqrt{x}</m> we should rewrite it
              in exponential form, i.e. as a power of <m>x</m>:
              <me>
                6\sqrt{x}=6x^{1/2}
              </me>
              It's very important that you become comfortable with fractional
              exponents: fractional exponents mean you have a root.  

              Now we can take the derivative:
              <md>
                <mrow>f' (x) \amp  = \ddx 6\sqrt{x}</mrow>
                <mrow>\amp  = \ddx 6x^{1/2}</mrow>
                <mrow>\amp  = 6\cdot \frac 12 x^{\tfrac 12 -1}</mrow>
                <mrow>\amp  = 3x^{-1/2} \text{ or }  \frac{3}{\sqrt{x}}</mrow>
              </md>
            </p>
          </li>

          <li>
            <p>
              Before taking the derivative of <m>\frac{5}{q^3}</m> we should 
              rewrite it in an exponential form,
              i.e.<nbsp />as a constant times a
              power of <m>q</m>:
              <me>
                \frac{5}{q^3} = 5q^{-3}
              </me>
              It's very important that you become comfortable with negative
              exponents: negative exponents mean you have
              <q>one over <ellipsis /></q>.

              Now we can take the derivative:
              <md>
                <mrow>C'(q) \amp  = \ddq (q^{13}-\frac{5}{q^3}+7)</mrow>
                <mrow>\amp  = \ddq (q^{13} -5q^{-3}+7)</mrow>
                <mrow>\amp  = 13q^{13-1} -5(-3)q^{-3-1}+0</mrow>
                <mrow>\amp  = 13q^{12} +15 q^{-4} \text{ or }  13q^{12}+\frac{15}{q^4}</mrow>
              </md>
            </p>
          </li>
        </ol>
      </p>
    </solution>
  </example>

  <example>
    <statement>
      <ol>
        <li>
          <p>
            For <m>y=2.5q^2-0.75q+9.23</m>, find <m>y''</m>.
          </p>
        </li>

        <li>
          <p>
            For <m>C(q) = q(q^2+q^{-2})</m>, find <m>C''(q)</m>.
          </p>
        </li>
      </ol>
    </statement>
    <solution>
      <p>
        <ol>
          <li>
            <p>
              <md>
                <mrow>y ' \amp  = \ddq (2.5q^2-0.75q+9.23)</mrow>
                <mrow>\amp  = 2.5(2)q^{2-1}-0.75(1)q^{0}+0\amp \amp  \text{ clean up before taking next derivative }</mrow>
                <mrow>\amp  = 5q-0.75</mrow>
                <mrow>y'' \amp  = \ddq (5q-0.75)</mrow>
                <mrow>\amp  = 5</mrow>
              </md>
            </p>
          </li>

          <li>
            <p>
              In this case we should <q>clean up</q> <em>before</em>
              you take even the first derivative:
              <me>
                C(q) = q(q^2+q^{-2}) = q^3+q^{-1}
              </me>
              Now we take derivatives:
              <md>
                <mrow>C'(q) \amp  = \ddq (q^3+q^{-1})</mrow>
                <mrow>\amp  = 3q^2 + (-1) q^{-1-1}</mrow>
                <mrow>\amp  = 3q^2 - q^{-2}</mrow>
                <mrow>C''(q) \amp  = 3(2)q^{1}-(-2)q^{-2-1}</mrow>
                <mrow>\amp  = 6q+2q^{-3}</mrow>
              </md>
            </p>
          </li>
        </ol>
      </p>
    </solution>
  </example>

  <example>
    <statement>
      <p>
        Let <m>f(x) =3x^2-4x+1</m>.

        <ol>
          <li>
            <p>
              Find the equation of the tangent line to <m>f</m> at <m>(1,0)</m>
            </p>
          </li>

          <li>
            <p>
              Find when <m>f</m> has a horizontal tangent line.
            </p>
          </li>
        </ol>
      </p>
    </statement>
    <solution>
      <p>
        <ol>
          <li>
            <p>
              We will fill in the following equation
              <md>
                <mrow>y \amp  = m(x-x_0) + y_0</mrow>
                <mrow>x_0 \amp  = 1</mrow>
                <mrow>y_0 \amp  = 0</mrow>
                <mrow>m \amp  = f'(x_0) = f'(1)</mrow>
              </md>
              We start by taking the derivative,
              and then plug this into the equations above:
              <md>
                <mrow>f' (x) \amp  = \ddx (3x^2-4x+1)</mrow>
                <mrow>\amp  = 6x-4</mrow>
                <mrow>m \amp  = f'(1)</mrow>
                <mrow>\amp  = 6(1)-4 = 2</mrow>
                <mrow>y \amp  = 2(x-1)+0</mrow>
                <mrow>\amp  = 2x-2</mrow>
              </md>
              Just to double check, you can look at the graphs to see we got it right:
              <image width="56%" source="images/" />
            </p>
          </li>

          <li>
            <p>
              First we <q>rewrite</q>
              the question, at least in our heads:
              <md>
                <mrow>f \text{ has a horizontal tangent line }  \amp  = \text{ means the slope is \(0\) }</mrow>
                <mrow>\amp  = \text{ means } f'(x)=0</mrow>
              </md>
              Now we set this up as an equation and solve it:
              <md>
                <mrow>f'(x) \amp  = 0</mrow>
                <mrow>6x-4 \amp  = 0</mrow>
                <mrow>6x \amp  = 4</mrow>
                <mrow>x \amp  = 4/6 = 2/3</mrow>
              </md>
              Just to double check, you can look at the graphs to see we got it right:
              <image width="56%" source="images/" />
            </p>
          </li>
        </ol>
      </p>
    </solution>
  </example>
</section>

