

<section>
  <title>Quadratics</title>
  <example>
    <statement>
      <p>
        A quadratic function has the following form
        <me>
          y = ax^2+bx+c
        </me>
      </p>

      <p>
        Match the following quadratics with their graphs: see if you can do
        this without using your calculator.

        <ol>
          <li>
            <p>
              <m>y=x^2</m>
            </p>
          </li>

          <li>
            <p>
              <m>y=(x+2)^2</m>
            </p>
          </li>

          <li>
            <p>
              <m>y=x^2+2</m>
            </p>
          </li>

          <li>
            <p>
              <m>y=-2x^2-3x+5</m>
            </p>
          </li>

          <li>
            <p>
              <m>y=3x^2-3x-5</m>
            </p>
          </li>
        </ol>
      </p>

      <p>
        \begin{beforesolutions}
      </p>

      <p>
        { <image width="28%" source="images/" /> }
      </p>

      <p>
        { <image width="28%" source="images/" /> }
      </p>

      <p>
        { <image width="28%" source="images/" /> }
      </p>

      <p>
        { <image width="28%" source="images/" /> }
      </p>

      <p>
        { <image width="28%" source="images/" /> }
      </p>

      <p>
        \end{beforesolutions}
      </p>
    </statement>
    <solution>
      <p>
        <image width="28%" source="images/" />
      </p>

      <p>
        <image width="28%" source="images/" />
      </p>

      <p>
        <image width="28%" source="images/" />
      </p>

      <p>
        <image width="28%" source="images/" />
      </p>

      <p>
        <image width="28%" source="images/" />
      </p>
    </solution>
  </example>

  <example>
    <statement>
      <p>
        Factoring a quadratic means to write it as a product.
        Usually you
        shouldn't bother to factor a quadratic unless the <m>x^2</m>-coefficient
        equals <m>1</m>.
        In that case, you're trying to write it like this:
        <me>
          y=x^2+bx+c = (x+d)(x+e)
        </me>
      </p>

      <p>
        There are various tricks in finding <m>d</m> and <m>e</m>,
        but honestly, in this
        case, I usually just guess and check as follows: (1) guess two values,
        <m>d</m> and <m>e</m>,
        that multiply together to give you <m>c</m>, and then (2)
        check to see if they add up to <m>b</m>.
        Note: when I write <q><m>+b</m></q> and
        <q><m>+c</m></q> and say <q>add</q>
        I'm also including negative numbers in there.

        <ol>
          \itemsep=\fill

          <li>
            <p>
              Factor and solve <m>x^2+2x+1=0</m>.
            </p>
          </li>

          <li>
            <p>
              Factor and solve <m>x^2+3x+2=0</m>.
            </p>
          </li>

          <li>
            <p>
              Factor and solve <m>x^2-3x+2=0</m>.
            </p>
          </li>

          <li>
            <p>
              Factor and solve <m>x^2-x-2=0</m>.
            </p>
          </li>

          <li>
            <p>
              Factor and solve <m>x^2-x-12=0</m>.
            </p>
          </li>

          <li>
            <p>
              Factor and solve <m>x^2-8x+12=0</m>. \handoutfill
            </p>
          </li>
        </ol>
      </p>
    </statement>
    <solution>
      <p>
        <ol>
          <li>
            <p>
              <md>
                <mrow>x^2+2x+1 \amp  =0</mrow>
                <mrow>(x+1)(x+1) \amp  = 0</mrow>
                <mrow>x\amp  = -1</mrow>
              </md>
            </p>
          </li>

          <li>
            <p>
              <md>
                <mrow>x^2+3x+2 \amp  = 0</mrow>
                <mrow>(x+2)(x+1) \amp  = 0</mrow>
                <mrow>x \amp  = -2, -1</mrow>
              </md>
            </p>
          </li>

          <li>
            <p>
              <md>
                <mrow>x^2-3x+2 \amp  = 0</mrow>
                <mrow>(x-2)(x-1) \amp  = 0</mrow>
                <mrow>x \amp  = 1,2</mrow>
              </md>
            </p>
          </li>

          <li>
            <p>
              <md>
                <mrow>x^2-x-2 \amp  = 0</mrow>
                <mrow>(x-2)(x+1) \amp  =0</mrow>
                <mrow>x \amp  = -1,2</mrow>
              </md>
            </p>
          </li>

          <li>
            <p>
              <md>
                <mrow>x^2-x-12 \amp  = 0</mrow>
                <mrow>(x-4)(x+3) \amp  = 0</mrow>
                <mrow>x \amp  = -3,4</mrow>
              </md>
            </p>
          </li>

          <li>
            <p>
              <md>
                <mrow>x^2-8x+12 \amp  = 0</mrow>
                <mrow>(x-10)(x+2) \amp  = 0</mrow>
                <mrow>x=-2,10</mrow>
              </md>
            </p>
          </li>
        </ol>
      </p>
    </solution>
  </example>

  <example>
    <statement>
      <p>
        A lot of times it's not worth factoring a quadratic, or it may be
        impossible.
        In these cases, just use the quadratic formula
        <me>
          ax^2+bx+c = 0 
          \Longrightarrow  
          x = \frac{-b\pm \sqrt{b^2-4ac}}{2a}
        </me>
        <ol>
          \itemsep=\fill

          <li>
            <p>
              Apply the quadratic formula to <m>x^2-x-12=0</m>.
            </p>
          </li>

          <li>
            <p>
              Apply the quadratic formula to <m>2x^2+3x-2=0</m>. \handoutfill
            </p>
          </li>
        </ol>
      </p>
    </statement>
    <solution>
      <p>
        <ol>
          <li>
            <p>
              <md>
                <mrow>x \amp  = \frac{+1 \pm \sqrt{(-1)^2 -4(1)(-12)}}{2(1)}</mrow>
                <mrow>\amp  = \frac{1 \pm \sqrt{1+48}}{2}</mrow>
                <mrow>\amp  = \frac{1 \pm \sqrt{49}}{2}</mrow>
                <mrow>\amp  = \frac{1 \pm 7}{2}</mrow>
                <mrow>\amp  = \frac{8}{2}, \frac{-6}{2}</mrow>
                <mrow>\amp  = 4, -3</mrow>
              </md>
              (Note:
        this is the same as part (e) in the previous example.)
            </p>
          </li>

          <li>
            <p>
              <md>
                <mrow>x \amp  = \frac{-3 \pm \sqrt{(3)^2 -4(2)(-2)}}{2(2)}</mrow>
                <mrow>\amp  = \frac{-3 \pm \sqrt{9+16}}{4}</mrow>
                <mrow>\amp  = \frac{-3 \pm \sqrt{25}}{4}</mrow>
                <mrow>\amp  = \frac{-3 \pm 5}{4}</mrow>
                <mrow>\amp  = \frac{2}{4}, \frac{-8}{4}</mrow>
                <mrow>\amp  = 1/2, -2</mrow>
              </md>
            </p>
          </li>
        </ol>
      </p>
    </solution>
  </example>
</section>

